Remove Arguments sentences from Shareable instances #137

base/Free/Test/SharingHandlerTests.v
@@ -36,7 +36,8 @@ Definition evalNDM {A : Type} p
 (* Shortcut to evaluate a traced partial program to a result and a list 
    of logged messages. *)
 Definition evalTraceM {A : Type} p
-:= @collectMessages (option A) (run (runTracing (runTraceSharing (0,0) (runMaybe p)))).
+:= @collectMessages (option A) 
+   (run (runTracing (runTraceSharing (0,0) (runMaybe p)))).
 
 (* Non-deterministic integer. *)
 Definition coin (Shape : Type) (Pos : Shape -> Type)
@@ -106,7 +107,8 @@ Definition double {Shape : Type}
 = 0+0 ? 0+1 ? 1+0 ? 1+1
 = 0 ? 1 ? 1 ? 2
 *)
-Example exAddNoSharingND : evalND (double (addInteger _ _) coin) = [0%Z;1%Z;1%Z;2%Z].
+Example exAddNoSharingND : evalND (double (addInteger _ _) coin) 
+                           = [0%Z;1%Z;1%Z;2%Z].
 Proof. constructor. Qed.
 
 (*
@@ -175,7 +177,8 @@ trace "Nothing" Nothing + trace "Nothing" Nothing
    only be logged once and the result should be Nothing (i.e. None in Coq).
 *)
 Example exTraceNothingNoSharing
- : evalTraceM (double (addInteger _ _) traceNothing) = (None,["Nothing"%string]).
+ : evalTraceM (double (addInteger _ _) traceNothing) 
+   = (None,["Nothing"%string]).
 Proof. constructor. Qed.
 
 (*
@@ -207,7 +210,9 @@ in sx + sx
 = 0+0 ? 1+1
 = 0 ? 2
 *)
-Example exAddSharingND : evalND (doubleShared Cbneed (addInteger _ _) coin) = [0%Z;2%Z].
+Example exAddSharingND : evalND (doubleShared (Cbneed Shape Pos _) 
+  (addInteger _ _) coin) 
+  = [0%Z;2%Z].
 Proof. constructor. Qed.
 
 (*
@@ -216,7 +221,8 @@ in sx + sx
 => The message should be logged once and the result should be 2.
 *)
 Example exAddSharingTrace 
- : evalTracing (doubleShared Cbneed (addInteger _ _) traceOne) = (2%Z,["One"%string]).
+ : evalTracing (doubleShared (Cbneed _ _ _) (addInteger _ _) traceOne) 
+ = (2%Z,["One"%string]).
 Proof. constructor. Qed.
 
 (*
@@ -226,7 +232,7 @@ in sx or sx
 = true ? false
 *)
 Example exOrNDSharing
- : evalND (doubleShared Cbneed (orBool _ _) coinB) = [true;false].
+ : evalND (doubleShared (Cbneed _ _ _) (orBool _ _) coinB) = [true;false].
 Proof. constructor. Qed.
 
 (*
@@ -236,7 +242,8 @@ in sx or sx
    The message should be logged once and the result should be true.
 *)
 Example exOrTrueTraceSharing
- : evalTracing (doubleShared Cbneed (orBool _ _) traceTrue) = (true,["True"%string]).
+ : evalTracing (doubleShared (Cbneed _ _ _) (orBool _ _) traceTrue)
+   = (true,["True"%string]).
 Proof. constructor. Qed.
 
 (*
@@ -246,7 +253,8 @@ in sx or sx
 only be logged once and the result should be false.
 *)
 Example exOrFalseTraceSharing
- : evalTracing (doubleShared Cbneed (orBool _ _) traceFalse) = (false,["False"%string]).
+ : evalTracing (doubleShared (Cbneed _ _ _) (orBool _ _) traceFalse)
+   = (false,["False"%string]).
 Proof. constructor. Qed.
 
 (* traceFalse is shared, but does not occur more than once. 
@@ -264,7 +272,8 @@ in sx + sx
 = Nothing ? Just 2
 *)
 Example exNDMSharing
- : evalNDM (doubleShared Cbneed (addInteger _ _) coinM) = [None;Some 2%Z].
+ : evalNDM (doubleShared (Cbneed _ _ _) (addInteger _ _) coinM)
+   = [None;Some 2%Z].
 Proof. constructor. Qed.
 
 (*
@@ -274,7 +283,8 @@ in sx + sx
    due to >>=.
 *)
 Example exTraceNothingSharing
- : evalTraceM (doubleShared Cbneed (addInteger _ _) traceNothing) = (None,["Nothing"%string]).
+ : evalTraceM (doubleShared (Cbneed _ _ _) (addInteger _ _) traceNothing)
+   = (None,["Nothing"%string]).
 Proof. constructor. Qed.
 
 (*
@@ -284,7 +294,8 @@ in sx + sx
    should be Some 2.
 *)
 Example exTraceJustSharing
- : evalTraceM (doubleShared Cbneed (addInteger _ _) traceJust) = (Some 2%Z,["Just 1"%string]).
+ : evalTraceM (doubleShared (Cbneed _ _ _) (addInteger _ _) traceJust)
+   = (Some 2%Z,["Just 1"%string]).
 Proof. constructor. Qed.
 
 (* --------------------- Test cases for nested sharing --------------------- *)
@@ -311,8 +322,10 @@ in sy + sy
 = (0+0)+(0+0) ? (1+1)+(1+1) 
 = 0 ? 4 
 *)
-Example exAddNestedSharingND : evalND (doubleSharedNested Cbneed (addInteger _ _) coin) 
-                            = [0%Z;4%Z].
+Example exAddNestedSharingND : evalND (doubleSharedNested (Cbneed _ _ _)
+                                                          (addInteger _ _) 
+                                                          coin) 
+                               = [0%Z;4%Z].
 Proof. constructor. Qed.
 
 (* 
@@ -322,7 +335,7 @@ in sy + sy
 => The message should only be logged once and the result should be 4. 
 *)
 Example exAddNestedSharingTrace 
- : evalTracing (doubleSharedNested Cbneed (addInteger _ _) traceOne) 
+ : evalTracing (doubleSharedNested (Cbneed _ _ _) (addInteger _ _) traceOne) 
    = (4%Z,["One"%string]).
 Proof. constructor. Qed.
 
@@ -333,7 +346,7 @@ in sy or sy
 = true ? false
 *)
 Example exOrNestedSharingND
- : evalND (doubleSharedNested Cbneed (orBool _ _) coinB)
+ : evalND (doubleSharedNested (Cbneed _ _ _) (orBool _ _) coinB)
    = [true;false].
 Proof. constructor. Qed.
 
@@ -345,7 +358,7 @@ in sy or sy
    and the result should be true.
 *)
 Example exOrNestedTrueTracing 
- : evalTracing (doubleSharedNested Cbneed (orBool _ _) traceTrue)
+ : evalTracing (doubleSharedNested (Cbneed _ _ _) (orBool _ _) traceTrue)
    = (true,["True"%string]).
 Proof. constructor. Qed.
 
@@ -357,7 +370,7 @@ in sy or sy
    and the result should be false.
 *)
 Example exOrNestedFalseTracing
- : evalTracing (doubleSharedNested Cbneed (orBool _ _) traceFalse)
+ : evalTracing (doubleSharedNested (Cbneed _ _ _) (orBool _ _) traceFalse)
    = (false, ["False"%string]).
 Proof. constructor. Qed.
 
@@ -389,7 +402,8 @@ in sy + sz
 = 0 ? 1 ? 2 ? 3
 *)
 Example exAddClashSharingND
- : evalND (doubleSharedClash Cbneed (addInteger _ _) coin coin) = [0%Z;1%Z;2%Z;3%Z].
+ : evalND (doubleSharedClash (Cbneed _ _ _) (addInteger _ _) coin coin) 
+   = [0%Z;1%Z;2%Z;3%Z].
 Proof. constructor. Qed.
 
 (*
@@ -400,7 +414,8 @@ in sy + sz
 => The message should be logged twice and the result should be 3.
 *)
 Example exAddClashSharingTracing
- : evalTracing (doubleSharedClash Cbneed (addInteger _ _) traceOne traceOne) 
+ : evalTracing (doubleSharedClash (Cbneed _ _ _) (addInteger _ _)
+                                  traceOne traceOne) 
    = (3%Z,["One"%string;"One"%string]).
 Proof. constructor. Qed.
 
@@ -414,7 +429,7 @@ in sy or sz
 = true ? true ? false
 *)
 Example exOrClashSharingND
- : evalND (doubleSharedClash Cbneed (orBool _ _) coinB coinB)
+ : evalND (doubleSharedClash (Cbneed _ _ _) (orBool _ _) coinB coinB)
    = [true;true;false].
 Proof. constructor. Qed.
 
@@ -427,7 +442,8 @@ in sy or sz
    result should be true.
 *)
 Example exOrClashTrueTracing
- : evalTracing (doubleSharedClash Cbneed (orBool _ _) traceTrue traceTrue)
+ : evalTracing (doubleSharedClash (Cbneed _ _ _) (orBool _ _)
+                                  traceTrue traceTrue)
    = (true,["True"%string]).
 Proof. constructor. Qed.
 
@@ -441,7 +457,8 @@ in sy or sz
    be logged twice in total and the result should be false.
 *)
 Example exOrClashFalseTracing
- : evalTracing (doubleSharedClash Cbneed (orBool _ _) traceFalse traceFalse)
+ : evalTracing (doubleSharedClash (Cbneed _ _ _) (orBool _ _)
+                                  traceFalse traceFalse)
    = (false,["False"%string;"False"%string]).
 Proof. constructor. Qed.
 
@@ -481,8 +498,10 @@ in sx + (sy + (sz + 1))
   ? (1 + (1+1 + ((1+1 + 1) + 1)))
 = 4 ? 5 ? 6 ? 7
 *)
-Example exAddRecSharingND : evalND (doubleSharedRec Cbneed (addInteger _ _) coin coin 1%Z) 
-                         = [4%Z;5%Z;6%Z;7%Z].
+Example exAddRecSharingND : evalND (doubleSharedRec (Cbneed _ _ _)
+                                                    (addInteger _ _) 
+                                                    coin coin 1%Z) 
+                            = [4%Z;5%Z;6%Z;7%Z].
 Proof. constructor. Qed.
 
 (*
@@ -496,7 +515,8 @@ in sx + (sy + (sz + 1))
    final value should be 1 + 2 + 3 + 1 = 7.
 *)
 Example exAddRecSharingTracing
- : evalTracing (doubleSharedRec Cbneed (addInteger _ _) traceOne traceOne 1%Z) 
+ : evalTracing (doubleSharedRec (Cbneed _ _ _) (addInteger _ _)
+                                traceOne traceOne 1%Z) 
    = (7%Z,["One"%string;"One"%string]).
 Proof. constructor. Qed.
 
@@ -508,7 +528,7 @@ in sx or (sy or (sz or true))
 = true (due to non-strictness)
 *)
 Example exOrRecSharingNDTrue
- : evalND (doubleSharedRec Cbneed (orBool _ _) coinB coinB true)
+ : evalND (doubleSharedRec (Cbneed _ _ _) (orBool _ _) coinB coinB true)
    = [true].
 Proof. constructor. Qed.
 
@@ -531,7 +551,7 @@ in sx or (sy or (sz or false))
 = true ? true ? false
 *)
 Example exOrRecSharingNDFalse
- : evalND (doubleSharedRec Cbneed (orBool _ _) coinB coinB false)
+ : evalND (doubleSharedRec (Cbneed _ _ _) (orBool _ _) coinB coinB false)
    = [true;true;false].
 Proof. constructor. Qed.
 
@@ -544,7 +564,8 @@ in sx or (sy or (sz or false))
    be logged once and the result should be true.
 *)
 Example exOrRecTrueTracing
- : evalTracing (doubleSharedRec Cbneed (orBool _ _) traceTrue traceTrue false)
+ : evalTracing (doubleSharedRec (Cbneed _ _ _) (orBool _ _)
+                                traceTrue traceTrue false)
    = (true,["True"%string]).
 Proof. constructor. Qed.
 
@@ -558,6 +579,7 @@ in sx or (sy or (sz or false))
    be false.
 *)
 Example exOrRecFalseTracing
- : evalTracing (doubleSharedRec Cbneed (orBool _ _) traceFalse traceFalse false)
+ : evalTracing (doubleSharedRec (Cbneed _ _ _) (orBool _ _)
+                                traceFalse traceFalse false)
    = (false,["False"%string;"False"%string]).
 Proof. constructor. Qed.
